src/lib/poly/Kuiper.Poly.AtomicReduce.fsti
@@ -9,22 +9,27 @@ open Kuiper.Atomics
 
 module SZ = Kuiper.SizeT
 
+noeq
+type is_ac_w (#t:Type) (f: t -> t -> t) = {
+  comm : (x:t -> y:t -> Lemma (f x y == f y x));
+  assoc : (x:t -> y:t -> z:t -> Lemma (f (f x y) z == f x (f y z)));
+}
+
 inline_for_extraction noextract
 type reduce_ty
   (et : Type0) {| scalar et |} {| d : has_atomic_add et |} =
+  (ac : is_ac_w d.pure_op) ->
   (n : szp{n < max_blocks}) ->
   (a : gpu_array et n { is_global_array a }) ->
-  (#f : perm) ->
   (#v_a : erased (seq et)) ->
   stt et
   (requires
     cpu **
-    pure (f == 1.0R) **
-    on gpu_loc (a |-> Frac f v_a) **
+    on gpu_loc (a |-> v_a) **
     pure (SZ.v n > 0 /\ SZ.v n <= 1024))
   (ensures fun r ->
     cpu **
-    on gpu_loc (a |-> Frac f v_a) **
+    on gpu_loc (a |-> v_a) **
     pure (r == Kuiper.Seq.Common.seq_fold_left d.pure_op zero v_a))
 
 inline_for_extraction noextract
